Hs.lean
@@ -3,3 +3,4 @@ import Hs.HsJudgment
 import Hs.Algorithm
 -- import Hs.CompileJ
 import Hs.Metatheory.Preservation2
+import Hs.Example
