Hs/Example.lean
@@ -2,6 +2,8 @@ import Hs.HsTerm
 import Hs.Algorithm
 import SystemFD.Algorithm
 
+import Aesop
+
 def idHsTerm : HsTerm := `λ{`#0} `#0
 def idHsType : HsTerm := `∀{`★} `#0 → `#1
 
@@ -11,12 +13,10 @@ def idTypeKinding : [] ⊢τ idHsType : `★ := by
   case _ => apply HsJudgment.ax (HsJudgment.wfnil)
   case _ =>
     apply HsJudgment.arrow;
-    case _ =>
-      apply HsJudgment.varTy; apply HsJudgment.wfkind; apply HsJudgment.ax (HsJudgment.wfnil);
+    apply HsJudgment.varTy; apply HsJudgment.wfkind; apply HsJudgment.ax (HsJudgment.wfnil);
       apply HsJudgment.wfnil; simp; unfold Frame.is_datatype; unfold Frame.apply; simp;
       unfold Frame.is_kind; simp; unfold Frame.get_type; unfold dnth; unfold Frame.apply; simp;
-    case _ =>
-      apply HsJudgment.varTy;
+    apply HsJudgment.varTy;
       apply HsJudgment.wfempty; apply HsJudgment.wfkind; apply HsJudgment.ax (HsJudgment.wfnil);
       apply HsJudgment.wfnil;
       simp; unfold Frame.is_kind; unfold Frame.apply; simp; unfold Frame.get_type; unfold dnth;
@@ -38,13 +38,13 @@ def idTyping : [] ⊢t idHsTerm : idHsType := by
    apply HsJudgment.wfnil; unfold Frame.is_type; unfold dnth; unfold Frame.apply; simp;
    unfold Frame.get_type; unfold dnth; unfold Frame.apply; simp;
    apply HsJudgment.arrow;
-   apply HsJudgment.varTy;
-   apply HsJudgment.wfkind; apply HsJudgment.ax (HsJudgment.wfnil); apply HsJudgment.wfnil;
-   unfold Frame.is_kind; unfold dnth; unfold Frame.apply; simp;
-   unfold Frame.get_type; unfold dnth; unfold Frame.apply; simp;
-   apply HsJudgment.varTy;
-   apply HsJudgment.wfempty;
-   apply HsJudgment.wfkind; apply HsJudgment.ax (HsJudgment.wfnil); apply HsJudgment.wfnil;
+     apply HsJudgment.varTy;
+     apply HsJudgment.wfkind; apply HsJudgment.ax (HsJudgment.wfnil); apply HsJudgment.wfnil;
+     unfold Frame.is_kind; unfold dnth; unfold Frame.apply; simp;
+     unfold Frame.get_type; unfold dnth; unfold Frame.apply; simp;
+     apply HsJudgment.varTy;
+     apply HsJudgment.wfempty;
+     apply HsJudgment.wfkind; apply HsJudgment.ax (HsJudgment.wfnil); apply HsJudgment.wfnil;
    unfold Frame.is_kind; unfold dnth; unfold Frame.apply; simp; unfold Frame.apply; simp;
    unfold Frame.get_type; unfold dnth; unfold Frame.apply; unfold dnth; simp; unfold Frame.apply; simp;
    apply HsJudgment.ax (HsJudgment.wfnil);
@@ -68,3 +68,592 @@ def idTerm := compile_term [] idHsTerm idHsType idTyping
 
 #eval idType
 #eval idTerm
+
+def MbCtx' : Ctx HsTerm :=
+  [ .ctor (`∀{`★} `#2 `•k `#0)   -- Nothing :: ∀ a. Maybe a
+  , .ctor (`∀{`★} `#0 → `#2 `•k `#1)          -- Just :: ∀ a. a -> Maybe a
+  , .datatype (`★ `-k> `★) ]
+
+def MbCtx : Ctx HsTerm :=
+  [ .ctor (`∀{`★} `#2 `•k `#0)   -- Nothing :: ∀ a. Maybe a
+  ,.ctor (`∀{`★} `#0 → `#2 `•k `#1)          -- Just :: ∀ a. a -> Maybe a
+  , .datatype (`★ `-k> `★) ]
+
+-- set_option trace.aesop.tree true
+-- set_option trace.aesop true
+attribute [aesop norm] Option.bind_eq_some
+def MaybeCtx : HsCtx MbCtx :=
+  .ctor
+    (.ctor
+      (.datatype .nil ⟨`★ `-k> `★ ,
+        by apply HsJudgment.arrowk; apply HsJudgment.ax; apply HsJudgment.wfnil
+           apply HsJudgment.ax; apply HsJudgment.wfnil⟩)
+      ⟨`∀{`★} `#0 → `#2 `•k `#1,
+        by apply HsJudgment.allt
+           apply HsJudgment.ax
+           apply HsJudgment.wfdatatype
+           apply HsJudgment.arrowk
+           apply HsJudgment.ax
+           apply HsJudgment.wfnil
+           apply HsJudgment.ax
+           apply HsJudgment.wfnil
+           apply HsJudgment.wfnil
+           apply HsJudgment.arrow
+           apply HsJudgment.varTy
+           apply HsJudgment.wfkind
+           apply HsJudgment.ax
+           apply HsJudgment.wfdatatype
+           apply HsJudgment.arrowk
+           apply HsJudgment.ax
+           apply HsJudgment.wfnil
+           apply HsJudgment.ax
+           apply HsJudgment.wfnil
+           apply HsJudgment.wfnil
+           apply HsJudgment.wfdatatype
+           apply HsJudgment.arrowk
+           apply HsJudgment.ax
+           apply HsJudgment.wfnil
+           apply HsJudgment.ax
+           apply HsJudgment.wfnil
+           apply HsJudgment.wfnil
+           simp_all only [dnth, substType_HsTerm, Bool.or_eq_true]
+           apply Or.inr; rfl
+           simp_all only [dnth, substType_HsTerm, Frame.get_type_apply_commute]; rfl
+           apply HsJudgment.appk
+           apply HsJudgment.varTy
+           apply HsJudgment.wfempty
+           apply HsJudgment.wfkind
+           apply HsJudgment.ax
+           apply HsJudgment.wfdatatype
+           apply HsJudgment.arrowk
+           apply HsJudgment.ax
+           apply HsJudgment.wfnil
+           apply HsJudgment.ax
+           apply HsJudgment.wfnil
+           apply HsJudgment.wfnil
+           apply HsJudgment.wfdatatype
+           apply HsJudgment.arrowk;
+             apply HsJudgment.ax; apply HsJudgment.wfnil;
+             apply HsJudgment.ax; apply HsJudgment.wfnil;
+           apply HsJudgment.wfnil
+           simp_all only [dnth, substType_HsTerm, Bool.or_eq_true, Frame.apply_compose, Frame.apply]
+           simp; apply Or.inl; unfold Frame.is_datatype; simp
+           unfold Frame.get_type; unfold dnth; unfold dnth; simp;
+           simp_all only[Frame.apply_compose, Frame.apply]; simp; rfl;
+           apply HsJudgment.varTy
+           apply HsJudgment.wfempty
+           apply HsJudgment.wfkind
+           apply HsJudgment.ax
+           apply HsJudgment.wfdatatype
+           apply HsJudgment.arrowk
+           apply HsJudgment.ax
+           apply HsJudgment.wfnil
+           apply HsJudgment.ax
+           apply HsJudgment.wfnil
+           apply HsJudgment.wfnil
+           apply HsJudgment.wfdatatype
+           apply HsJudgment.arrowk
+           apply HsJudgment.ax
+           apply HsJudgment.wfnil
+           apply HsJudgment.ax
+           apply HsJudgment.wfnil
+           apply HsJudgment.wfnil
+           simp_all only [dnth, substType_HsTerm, Bool.or_eq_true]
+           apply Or.inr; rfl
+           simp_all only [dnth, substType_HsTerm, Frame.get_type_apply_commute, Option.map_map]; rfl
+      ⟩)
+    ⟨`∀{`★} `#2 `•k `#0, by
+      apply HsJudgment.allt
+      apply HsJudgment.ax;
+        apply HsJudgment.wfctor;
+        { apply HsJudgment.allt;
+          apply HsJudgment.ax
+          apply HsJudgment.wfdatatype
+          apply HsJudgment.arrowk
+          apply HsJudgment.ax
+          apply HsJudgment.wfnil
+          apply HsJudgment.ax
+          apply HsJudgment.wfnil
+          apply HsJudgment.wfnil
+          apply HsJudgment.arrow
+          apply HsJudgment.varTy
+          apply HsJudgment.wfkind
+          apply HsJudgment.ax
+          apply HsJudgment.wfdatatype
+          apply HsJudgment.arrowk
+          apply HsJudgment.ax
+          apply HsJudgment.wfnil
+          apply HsJudgment.ax
+          apply HsJudgment.wfnil
+          apply HsJudgment.wfnil
+          apply HsJudgment.wfdatatype
+          apply HsJudgment.arrowk
+          apply HsJudgment.ax
+          apply HsJudgment.wfnil
+          apply HsJudgment.ax
+          apply HsJudgment.wfnil
+          apply HsJudgment.wfnil
+          simp_all only [dnth, substType_HsTerm, Bool.or_eq_true]
+          apply Or.inr; rfl;
+          simp_all only [dnth, substType_HsTerm, Frame.get_type_apply_commute]; rfl;
+          apply HsJudgment.appk
+
+          apply HsJudgment.varTy
+          apply HsJudgment.wfempty
+          apply HsJudgment.wfkind
+          apply HsJudgment.ax
+          apply HsJudgment.wfdatatype
+          apply HsJudgment.arrowk
+          apply HsJudgment.ax
+          apply HsJudgment.wfnil
+          apply HsJudgment.ax
+          apply HsJudgment.wfnil
+          apply HsJudgment.wfnil
+          apply HsJudgment.wfdatatype
+          apply HsJudgment.arrowk
+          apply HsJudgment.ax
+          apply HsJudgment.wfnil
+          apply HsJudgment.ax
+          apply HsJudgment.wfnil
+          apply HsJudgment.wfnil
+          simp_all only [dnth, substType_HsTerm, Bool.or_eq_true]
+          apply Or.inl; rfl
+          simp_all only [dnth, substType_HsTerm, Frame.get_type_apply_commute, Option.map_map]; rfl;
+
+          -- simp_all only [Function.comp_apply, HsTerm.subst_const]
+          apply HsJudgment.varTy
+          apply HsJudgment.wfempty
+          apply HsJudgment.wfkind
+          apply HsJudgment.ax
+          apply HsJudgment.wfdatatype
+          apply HsJudgment.arrowk
+          apply HsJudgment.ax
+          apply HsJudgment.wfnil
+          apply HsJudgment.ax
+          apply HsJudgment.wfnil
+          apply HsJudgment.wfnil
+          apply HsJudgment.wfdatatype
+          apply HsJudgment.arrowk
+          apply HsJudgment.ax
+          apply HsJudgment.wfnil
+          apply HsJudgment.ax
+          apply HsJudgment.wfnil
+          apply HsJudgment.wfnil
+          simp_all only [dnth, substType_HsTerm, Bool.or_eq_true, Frame.apply, Frame.is_kind]
+          apply Or.inr; simp;
+          simp_all only [dnth, Frame.get_type_apply_commute, Option.map_map, Frame.get_type];
+          unfold Frame.apply; simp};
+        apply HsJudgment.wfdatatype;   apply HsJudgment.arrowk; apply HsJudgment.ax;
+        apply HsJudgment.wfnil; apply HsJudgment.ax; apply HsJudgment.wfnil; apply HsJudgment.wfnil;
+        apply ValidHsCtorType.all; apply ValidHsCtorType.arrow; apply ValidHsCtorType.refl;
+        unfold HsValidHeadVariable; simp; rfl
+      apply HsJudgment.appk;
+        apply HsJudgment.varTy;
+          apply HsJudgment.wfkind;
+            apply HsJudgment.ax;
+            {
+              apply HsJudgment.wfctor;
+              {
+                apply HsJudgment.allt
+                · apply HsJudgment.ax
+                  apply HsJudgment.wfdatatype
+                  · apply HsJudgment.arrowk
+                    · apply HsJudgment.ax
+                      apply HsJudgment.wfnil
+                    · apply HsJudgment.ax
+                      apply HsJudgment.wfnil
+                  · apply HsJudgment.wfnil
+                · apply HsJudgment.arrow
+                  · apply HsJudgment.varTy
+                    · apply HsJudgment.wfkind
+                      · apply HsJudgment.ax
+                        apply HsJudgment.wfdatatype
+                        · apply HsJudgment.arrowk
+                          · apply HsJudgment.ax
+                            apply HsJudgment.wfnil
+                          · apply HsJudgment.ax
+                            apply HsJudgment.wfnil
+                        · apply HsJudgment.wfnil
+                      · apply HsJudgment.wfdatatype
+                        · apply HsJudgment.arrowk
+                          · apply HsJudgment.ax
+                            apply HsJudgment.wfnil
+                          · apply HsJudgment.ax
+                            apply HsJudgment.wfnil
+                        · apply HsJudgment.wfnil
+                    · simp_all only [dnth, substType_HsTerm, Bool.or_eq_true]
+                      apply Or.inr
+                      rfl
+                    · simp_all only [dnth, substType_HsTerm, Frame.get_type_apply_commute]
+                      rfl
+                  · apply HsJudgment.appk
+                    on_goal 2 => {
+                      apply HsJudgment.varTy
+                      · apply HsJudgment.wfempty
+                        apply HsJudgment.wfkind
+                        · apply HsJudgment.ax
+                          apply HsJudgment.wfdatatype
+                          · apply HsJudgment.arrowk
+                            · apply HsJudgment.ax
+                              apply HsJudgment.wfnil
+                            · apply HsJudgment.ax
+                              apply HsJudgment.wfnil
+                          · apply HsJudgment.wfnil
+                        · apply HsJudgment.wfdatatype
+                          · apply HsJudgment.arrowk
+                            · apply HsJudgment.ax
+                              apply HsJudgment.wfnil
+                            · apply HsJudgment.ax
+                              apply HsJudgment.wfnil
+                          · apply HsJudgment.wfnil
+                      · simp_all only [dnth, substType_HsTerm, Bool.or_eq_true]
+                        apply Or.inr
+                        rfl
+                      · simp_all only [dnth, substType_HsTerm, Frame.get_type_apply_commute, Option.map_map]
+                        rfl
+                    }
+                    · simp_all only [Function.comp_apply, HsTerm.subst_const]
+                      apply HsJudgment.varTy
+                      · apply HsJudgment.wfempty
+                        apply HsJudgment.wfkind
+                        · apply HsJudgment.ax
+                          apply HsJudgment.wfdatatype
+                          · apply HsJudgment.arrowk
+                            · apply HsJudgment.ax
+                              apply HsJudgment.wfnil
+                            · apply HsJudgment.ax
+                              apply HsJudgment.wfnil
+                          · apply HsJudgment.wfnil
+                        · apply HsJudgment.wfdatatype
+                          · apply HsJudgment.arrowk
+                            · apply HsJudgment.ax
+                              apply HsJudgment.wfnil
+                            · apply HsJudgment.ax
+                              apply HsJudgment.wfnil
+                          · apply HsJudgment.wfnil
+                      · simp_all only [dnth, substType_HsTerm, Bool.or_eq_true]
+                        apply Or.inl
+                        rfl
+                      · simp_all only [dnth, substType_HsTerm, Frame.get_type_apply_commute, Option.map_map]
+                        rfl
+
+              };
+              {
+                apply HsJudgment.wfdatatype
+                · apply HsJudgment.arrowk
+                  · apply HsJudgment.ax
+                    apply HsJudgment.wfnil
+                  · apply HsJudgment.ax
+                    apply HsJudgment.wfnil
+                · apply HsJudgment.wfnil
+              };
+              {
+                apply ValidHsCtorType.all; apply ValidHsCtorType.arrow;
+                apply ValidHsCtorType.refl; unfold HsValidHeadVariable; simp;
+                simp_all only [Frame.apply, Frame.is_datatype];
+              };
+
+            };
+            apply HsJudgment.wfctor;
+            apply HsJudgment.allt;
+            {
+                apply HsJudgment.ax
+                apply HsJudgment.wfdatatype
+                · apply HsJudgment.arrowk
+                  · apply HsJudgment.ax
+                    apply HsJudgment.wfnil
+                  · apply HsJudgment.ax
+                    apply HsJudgment.wfnil
+                · apply HsJudgment.wfnil
+            };
+            {
+                apply HsJudgment.arrow
+                · apply HsJudgment.varTy
+                  · apply HsJudgment.wfkind
+                    · apply HsJudgment.ax
+                      apply HsJudgment.wfdatatype
+                      · apply HsJudgment.arrowk
+                        · apply HsJudgment.ax
+                          apply HsJudgment.wfnil
+                        · apply HsJudgment.ax
+                          apply HsJudgment.wfnil
+                      · apply HsJudgment.wfnil
+                    · apply HsJudgment.wfdatatype
+                      · apply HsJudgment.arrowk
+                        · apply HsJudgment.ax
+                          apply HsJudgment.wfnil
+                        · apply HsJudgment.ax
+                          apply HsJudgment.wfnil
+                      · apply HsJudgment.wfnil
+                  · simp_all only [dnth, substType_HsTerm, Bool.or_eq_true]
+                    apply Or.inr
+                    rfl
+                  · simp_all only [dnth, substType_HsTerm, Frame.get_type_apply_commute]
+                    rfl
+                · apply HsJudgment.appk
+                  · apply HsJudgment.varTy
+                    · apply HsJudgment.wfempty
+                      apply HsJudgment.wfkind
+                      · apply HsJudgment.ax
+                        apply HsJudgment.wfdatatype
+                        · apply HsJudgment.arrowk
+                          · apply HsJudgment.ax
+                            apply HsJudgment.wfnil
+                          · apply HsJudgment.ax
+                            apply HsJudgment.wfnil
+                        · apply HsJudgment.wfnil
+                      · apply HsJudgment.wfdatatype
+                        · apply HsJudgment.arrowk
+                          · apply HsJudgment.ax
+                            apply HsJudgment.wfnil
+                          · apply HsJudgment.ax
+                            apply HsJudgment.wfnil
+                        · apply HsJudgment.wfnil
+                    · simp_all only [dnth, substType_HsTerm, Bool.or_eq_true]
+                      apply Or.inl
+                      rfl
+                    · simp_all only [dnth, substType_HsTerm, Frame.get_type_apply_commute, Option.map_map]
+                      rfl
+                  · simp_all only [HsTerm.smap, HsTerm.smap.eq_3]
+                    apply HsJudgment.varTy
+                    · apply HsJudgment.wfempty
+                      apply HsJudgment.wfkind
+                      · apply HsJudgment.ax
+                        apply HsJudgment.wfdatatype
+                        · apply HsJudgment.arrowk
+                          · apply HsJudgment.ax
+                            apply HsJudgment.wfnil
+                          · apply HsJudgment.ax
+                            apply HsJudgment.wfnil
+                        · apply HsJudgment.wfnil
+                      · apply HsJudgment.wfdatatype
+                        · apply HsJudgment.arrowk
+                          · apply HsJudgment.ax
+                            apply HsJudgment.wfnil
+                          · apply HsJudgment.ax
+                            apply HsJudgment.wfnil
+                        · apply HsJudgment.wfnil
+                    · simp_all only [dnth, substType_HsTerm, Bool.or_eq_true]
+                      apply Or.inr
+                      rfl
+                    · simp_all only [dnth, substType_HsTerm, Frame.get_type_apply_commute, Option.map_map]
+                      rfl
+            };
+            apply HsJudgment.wfdatatype;
+            apply HsJudgment.arrowk;
+            apply HsJudgment.ax; apply HsJudgment.wfnil;
+            apply HsJudgment.ax; apply HsJudgment.wfnil;
+            apply HsJudgment.wfnil;
+            apply ValidHsCtorType.all; apply ValidHsCtorType.arrow;
+            apply ValidHsCtorType.refl; unfold HsValidHeadVariable; simp;
+            simp_all only [Frame.apply, Frame.is_datatype];
+          simp; apply Or.inl; rfl;
+          unfold Frame.get_type; unfold dnth; unfold Frame.apply; unfold dnth;
+          simp; unfold Frame.apply; simp; rfl;
+        apply HsJudgment.varTy;
+          {apply HsJudgment.wfkind;
+            apply HsJudgment.ax;
+            {apply HsJudgment.wfctor;
+              {
+        apply HsJudgment.allt
+        · apply HsJudgment.ax
+          apply HsJudgment.wfdatatype
+          · apply HsJudgment.arrowk
+            · apply HsJudgment.ax
+              apply HsJudgment.wfnil
+            · apply HsJudgment.ax
+              apply HsJudgment.wfnil
+          · apply HsJudgment.wfnil
+        · apply HsJudgment.arrow
+          · apply HsJudgment.varTy
+            · apply HsJudgment.wfkind
+              · apply HsJudgment.ax
+                apply HsJudgment.wfdatatype
+                · apply HsJudgment.arrowk
+                  · apply HsJudgment.ax
+                    apply HsJudgment.wfnil
+                  · apply HsJudgment.ax
+                    apply HsJudgment.wfnil
+                · apply HsJudgment.wfnil
+              · apply HsJudgment.wfdatatype
+                · apply HsJudgment.arrowk
+                  · apply HsJudgment.ax
+                    apply HsJudgment.wfnil
+                  · apply HsJudgment.ax
+                    apply HsJudgment.wfnil
+                · apply HsJudgment.wfnil
+            · simp_all only [dnth, substType_HsTerm, Bool.or_eq_true]
+              apply Or.inr
+              rfl
+            · simp_all only [dnth, substType_HsTerm, Frame.get_type_apply_commute]
+              rfl
+          · apply HsJudgment.appk
+            on_goal 2 => {
+              apply HsJudgment.varTy
+              · apply HsJudgment.wfempty
+                apply HsJudgment.wfkind
+                · apply HsJudgment.ax
+                  apply HsJudgment.wfdatatype
+                  · apply HsJudgment.arrowk
+                    · apply HsJudgment.ax
+                      apply HsJudgment.wfnil
+                    · apply HsJudgment.ax
+                      apply HsJudgment.wfnil
+                  · apply HsJudgment.wfnil
+                · apply HsJudgment.wfdatatype
+                  · apply HsJudgment.arrowk
+                    · apply HsJudgment.ax
+                      apply HsJudgment.wfnil
+                    · apply HsJudgment.ax
+                      apply HsJudgment.wfnil
+                  · apply HsJudgment.wfnil
+              · simp_all only [dnth, substType_HsTerm, Bool.or_eq_true]
+                apply Or.inr
+                rfl
+              · simp_all only [dnth, substType_HsTerm, Frame.get_type_apply_commute, Option.map_map]
+                rfl
+            }
+            · simp_all only [Function.comp_apply, HsTerm.subst_const]
+              apply HsJudgment.varTy
+              · apply HsJudgment.wfempty
+                apply HsJudgment.wfkind
+                · apply HsJudgment.ax
+                  apply HsJudgment.wfdatatype
+                  · apply HsJudgment.arrowk
+                    · apply HsJudgment.ax
+                      apply HsJudgment.wfnil
+                    · apply HsJudgment.ax
+                      apply HsJudgment.wfnil
+                  · apply HsJudgment.wfnil
+                · apply HsJudgment.wfdatatype
+                  · apply HsJudgment.arrowk
+                    · apply HsJudgment.ax
+                      apply HsJudgment.wfnil
+                    · apply HsJudgment.ax
+                      apply HsJudgment.wfnil
+                  · apply HsJudgment.wfnil
+              · simp_all only [dnth, substType_HsTerm, Bool.or_eq_true]
+                apply Or.inl
+                rfl
+              · simp_all only [dnth, substType_HsTerm, Frame.get_type_apply_commute, Option.map_map]
+                rfl};
+              apply HsJudgment.wfdatatype;
+              apply HsJudgment.arrowk;
+              apply HsJudgment.ax;
+              apply HsJudgment.wfnil;
+              apply HsJudgment.ax;
+              apply HsJudgment.wfnil;
+              apply HsJudgment.wfnil;
+              {
+                apply ValidHsCtorType.all; apply ValidHsCtorType.arrow;
+                apply ValidHsCtorType.refl; unfold HsValidHeadVariable; simp;
+                simp_all only [Frame.apply, Frame.is_datatype];
+              }
+            };
+            {apply HsJudgment.wfctor;
+              {
+
+        apply HsJudgment.allt
+        · apply HsJudgment.ax
+          apply HsJudgment.wfdatatype
+          · apply HsJudgment.arrowk
+            · apply HsJudgment.ax
+              apply HsJudgment.wfnil
+            · apply HsJudgment.ax
+              apply HsJudgment.wfnil
+          · apply HsJudgment.wfnil
+        · apply HsJudgment.arrow
+          · apply HsJudgment.varTy
+            · apply HsJudgment.wfkind
+              · apply HsJudgment.ax
+                apply HsJudgment.wfdatatype
+                · apply HsJudgment.arrowk
+                  · apply HsJudgment.ax
+                    apply HsJudgment.wfnil
+                  · apply HsJudgment.ax
+                    apply HsJudgment.wfnil
+                · apply HsJudgment.wfnil
+              · apply HsJudgment.wfdatatype
+                · apply HsJudgment.arrowk
+                  · apply HsJudgment.ax
+                    apply HsJudgment.wfnil
+                  · apply HsJudgment.ax
+                    apply HsJudgment.wfnil
+                · apply HsJudgment.wfnil
+            · simp_all only [dnth, substType_HsTerm, Bool.or_eq_true]
+              apply Or.inr
+              rfl
+            · simp_all only [dnth, substType_HsTerm, Frame.get_type_apply_commute]
+              rfl
+          · apply HsJudgment.appk
+            on_goal 2 => {
+              apply HsJudgment.varTy
+              · apply HsJudgment.wfempty
+                apply HsJudgment.wfkind
+                · apply HsJudgment.ax
+                  apply HsJudgment.wfdatatype
+                  · apply HsJudgment.arrowk
+                    · apply HsJudgment.ax
+                      apply HsJudgment.wfnil
+                    · apply HsJudgment.ax
+                      apply HsJudgment.wfnil
+                  · apply HsJudgment.wfnil
+                · apply HsJudgment.wfdatatype
+                  · apply HsJudgment.arrowk
+                    · apply HsJudgment.ax
+                      apply HsJudgment.wfnil
+                    · apply HsJudgment.ax
+                      apply HsJudgment.wfnil
+                  · apply HsJudgment.wfnil
+              · simp_all only [dnth, substType_HsTerm, Bool.or_eq_true]
+                apply Or.inr
+                rfl
+              · simp_all only [dnth, substType_HsTerm, Frame.get_type_apply_commute, Option.map_map]
+                rfl
+            }
+            · simp_all only [Function.comp_apply, HsTerm.subst_const]
+              apply HsJudgment.varTy
+              · apply HsJudgment.wfempty
+                apply HsJudgment.wfkind
+                · apply HsJudgment.ax
+                  apply HsJudgment.wfdatatype
+                  · apply HsJudgment.arrowk
+                    · apply HsJudgment.ax
+                      apply HsJudgment.wfnil
+                    · apply HsJudgment.ax
+                      apply HsJudgment.wfnil
+                  · apply HsJudgment.wfnil
+                · apply HsJudgment.wfdatatype
+                  · apply HsJudgment.arrowk
+                    · apply HsJudgment.ax
+                      apply HsJudgment.wfnil
+                    · apply HsJudgment.ax
+                      apply HsJudgment.wfnil
+                  · apply HsJudgment.wfnil
+              · simp_all only [dnth, substType_HsTerm, Bool.or_eq_true]
+                apply Or.inl
+                rfl
+              · simp_all only [dnth, substType_HsTerm, Frame.get_type_apply_commute, Option.map_map]
+                rfl
+              };
+              { apply HsJudgment.wfdatatype
+                · apply HsJudgment.arrowk
+                  · apply HsJudgment.ax
+                    apply HsJudgment.wfnil
+                  · apply HsJudgment.ax
+                    apply HsJudgment.wfnil
+                · apply HsJudgment.wfnil };
+              {
+                apply ValidHsCtorType.all; apply ValidHsCtorType.arrow;
+                apply ValidHsCtorType.refl; unfold HsValidHeadVariable; simp;
+                simp_all only [Frame.apply, Frame.is_datatype]
+              }
+          }};
+          { simp_all only [dnth, substType_HsTerm, Bool.or_eq_true]; apply Or.inr; rfl};
+          {simp_all only [dnth, substType_HsTerm, Bool.or_eq_true]; rfl};
+    ⟩
+
+#eval compile_ctx MaybeCtx
+#guard compile_ctx MaybeCtx == .some [ .ctor (∀[★](#2 `@k #0))
+                                     , .ctor (∀[★]#0 -t> (#2 `@k #1))
+                                     , .datatype (★ -k> ★)]
