Hs/Metatheory/Preservation2.lean
@@ -1,25 +1,25 @@
 import Hs.Algorithm
 
-inductive HsKindLike : HsTerm -> Prop where
-| HsType : HsKindLike `★
-| HsArrK : HsKindLike k -> HsKindLike k' -> HsKindLike (k `-k> k')
-
 inductive CompileCtx : Ctx HsTerm -> Ctx Term -> Prop where
 | nil : CompileCtx [] []
 | empty :
+  ⊢s Γ ->
   CompileCtx Γ Γ' ->
   CompileCtx (.empty :: Γ) (.empty :: Γ')
 | kind :
+  ⊢s Γ ->
   CompileCtx Γ Γ' ->
   (j1 : Γ ⊢κ A : `□) ->
   compile_kind Γ A `□ j1 = .some A' ->
   CompileCtx (.kind A :: Γ) (.kind A' :: Γ')
 | type :
+  ⊢s Γ ->
   CompileCtx Γ Γ' ->
   (j1 : Γ ⊢τ A : `★) ->
   compile_type Γ A `★ j1 = .some A' ->
   CompileCtx (.type A :: Γ) (.type A' :: Γ')
 | term :
+  ⊢s Γ ->
   CompileCtx Γ Γ' ->
   (j1 : Γ ⊢τ A : `★)  ->
   (j2 : Γ ⊢t t : τ) ->
@@ -27,71 +27,62 @@ inductive CompileCtx : Ctx HsTerm -> Ctx Term -> Prop where
   compile_term Γ t τ j2 = .some t' ->
   CompileCtx (.term A t :: Γ) (.term A' t' :: Γ')
 
-theorem compile_preserves_indices :
+theorem compile_ctx_type :
   CompileCtx Γ Γ' ->
-  (j2 : Γ ⊢κ  T : `□) ->
-  (j1 : Γ ⊢τ `#x : T) ->
-  compile_kind Γ T `□ j = .some T' ->
+  (Γ d@ x).get_type = .some τ ->
+  (j : Γ ⊢τ `#x : τ) ->
+  compile_type Γ `#x τ j = .some τ' ->
+  (Γ' @ x).get_type = .some τ' :=
+by
+intro cc gt j c;
+unfold compile_type at c; cases j; cases c;
+case _ wf test gt =>
+ clear gt;
+ induction cc;
+ case _ => cases test
+ case _ =>
+   induction x generalizing Γ Γ';
+   case _ => cases gt;
+   case _ ih1 ih2 =>
+   sorry
+ case _ => sorry
+ case _ => sorry
+ case _ => sorry
+
+
+theorem compile_preserves_term_indices :
+  CompileCtx Γ Γ' ->
+  (j1 : Γ ⊢t `#x : T) ->
+  compile_type Γ T k j = .some T' ->
   (Γ' d@ x).get_type = .some T' := by
-intro cc j1 j2 ct;
-cases j2;
-induction cc;
-case _ wf h gt => unfold Frame.get_type at gt; simp at gt;
-case _ wf h gt => sorry
-case _ => sorry
-case _ => sorry
-case _ => sorry
-
-
-
-theorem compile_ctx_wf :
-  ⊢s Γ ->
-  CompileCtx Γ Γ' ->
-  ⊢ Γ' := by
-intro h1 h2;
-induction h2;
-case _ => apply Judgment.wfnil
-case _ h1 ih1 =>
-  cases h1; case _ h1 =>
-  apply Judgment.wfempty;
-  apply ih1 h1;
-case _ h1 j1 cc ih =>
- apply Judgment.wfkind;
- sorry
- sorry
-case _ => sorry
-case _ => sorry
+sorry
 
 theorem kinding_uniqueness :
-  HsKindLike τ ->
   Γ ⊢κ τ : k ->
   Γ ⊢κ τ : k' ->
   k = k' :=
  by
-intro h j1 j2
+intro j1 j2
 induction τ generalizing Γ k k'
-all_goals (cases h)
 case _ => cases j1; cases j2; rfl
+all_goals (cases j1)
 case _ ih1 ih2 kl1 kl2 =>
-  cases j1; cases j2; rfl;
+  cases j2; rfl;
 
 theorem compile_preserves_kinds :
-  HsKindLike t ->
-  τ = `□ ->
+  CompileCtx Γ Γ' ->
   (j : Γ ⊢κ t : τ) ->
   compile_kind Γ t τ j = .some t' ->
-  CompileCtx Γ Γ' ->
   Γ' ⊢ t' : .kind := by
- intro h e j c cc;
+ intro cc j c;
  induction Γ, t, τ, j using compile_kind.induct generalizing t'
  all_goals try (cases e)
- all_goals try (cases h)
  case _ =>
    unfold compile_kind at c; cases c;
-   case _ wf =>
-     apply Judgment.ax;
-     apply compile_ctx_wf wf cc
- case _ j1 j2 ih1 ih2 kl1 kl2 =>
+   case _ wf => sorry
+     -- apply Judgment.ax;
+     -- apply compile_ctx_wf wf cc
+ case _ j1 j2 ih1 ih2 =>
    unfold compile_kind at c; simp at c;
    rw[Option.bind_eq_some] at c;
    cases c; case _ w1 c1 =>
@@ -100,61 +91,69 @@ theorem compile_preserves_kinds :
    cases c2; case _ w2 c2 =>
    cases c2; case _ c2 c3 =>
    cases c3;
-   have ih1' := @ih1 w1 kl1 rfl c1 cc;
-   have ih2' := @ih2 w2 kl2 rfl c2 cc;
+   have ih1' := @ih1 w1 cc c1;
+   have ih2' := @ih2 w2 cc c2;
    apply Judgment.allk;
    apply ih1';
    apply ih2'
 
-inductive HsTypeLike : Ctx HsTerm -> HsTerm -> Prop where
-| HsArr : HsTypeLike Γ τ -> HsTypeLike (.empty::Γ) τ' -> HsTypeLike Γ (τ → τ')
-| HsFArr : HsTypeLike Γ τ -> HsTypeLike (.empty::Γ) τ' -> HsTypeLike Γ (τ ⇒ τ')
-| HsVarTy : (Γ d@x).is_datatype || (Γ d@ x).is_kind -> HsTypeLike Γ (`#x)
-| HsAll : HsKindLike A -> HsTypeLike (.kind A::Γ) τ -> HsTypeLike Γ (`∀{A} τ)
+
+def typing_js_gives_kinding_js :
+  Γ ⊢τ t : k ->
+  Γ ⊢κ k : `□ := by
+intro j; sorry
+
 
 theorem typing_uniqueness :
-  HsTypeLike Γ t ->
   Γ ⊢τ t : k ->
   Γ ⊢τ t : k' ->
   k = k' := by
-intro h j1 j2;
-induction t generalizing Γ;
-all_goals (cases h)
+intro j1 j2;
+induction t generalizing Γ k k';
+all_goals (cases j1)
 case _ =>
-  cases j1; cases j2
+  cases j2
   case _ h2 _ _ h1 =>
   rw [<-h1] at h2; injection h2;
-case _ =>
-  cases j1; cases j2;
-  case _ tl1 _ j1 _ _ j2 _ _ ih1 _ =>
-  apply ih1 tl1 j1 j2
-case _ =>
-  cases j1; cases j2;
-  case _ tl1 _ j1 _ _ j2 _ _ ih1 _ =>
-  apply ih1 tl1 j1 j2
-case _ =>
-  cases j1; cases j2;
-  case _ j2 _ _ _ j1 _ ih =>
-  apply ih j2 j1 j1
+all_goals(cases j2)
+case _ ih1 ih2 A j1 j2 A' j1' j2' =>
+  have u := @ih2 Γ A A' j1 j1'; subst u;
+  have u := @ih1 Γ (A `-k> k) (A `-k> k') j2 j2';
+  simp at u; apply u;
+case _ => rfl
+case _ => rfl
+case _ => rfl
 
 theorem compile_preserves_types :
-  HsKindLike k ->
+  CompileCtx Γ Γ' ->
   (j2 : Γ ⊢κ k : `□) ->
   compile_kind Γ k `□ j2 = .some k' ->
-  HsTypeLike Γ τ ->
   (j1 : Γ ⊢τ τ : k) ->
   compile_type Γ τ k j1 = .some τ' ->
-  CompileCtx Γ Γ' ->
   Γ' ⊢ τ' : k' := by
-intro kl j1 c1 tl j2 c2 cc;
+intro cc j1 c1 j2 c2;
 induction Γ, τ, k, j2 using compile_type.induct generalizing Γ' τ' k'
 all_goals (unfold compile_type at c2; simp at c2)
-case _ =>
-  cases c2;
-  apply Judgment.var;
-  apply compile_ctx_wf; assumption; assumption;
-  sorry
-case _ h1 h2 ih1 ih2 => cases tl
+case _ Γ x wf test gt =>
+     cases c2; sorry
+  -- cases c2;
+  -- apply Judgment.var;
+  -- apply compile_ctx_wf; assumption; assumption;
+  -- have lem1 := HsJudgment.varTy wf test gt
+  -- have lem := compile_preserves_type_indices cc lem1 c1; symm at lem;
+  -- assumption
+case _ h1 h2 ih1 ih2 =>
+  rw[Option.bind_eq_some] at c2;
+  cases c2; case _ w1 c2 =>
+  cases c2; case _ c2 c3 =>
+  rw[Option.bind_eq_some] at c3;
+  cases c3; case _ w2 c3 =>
+  cases c3; case _ c3 e =>
+  cases e;
+  apply Judgment.appk;
+  case _ => sorry;
+  case _ => sorry;
+  case _ => sorry
 case _ h1 h2 ih1 =>
   rw[Option.bind_eq_some] at c2;
   cases c2; case _ w1 c2 =>
@@ -164,13 +163,13 @@ case _ h1 h2 ih1 =>
   cases c3; case _ c3 e =>
   cases e; unfold compile_kind at c1; cases j1;
   simp at c1; cases c1;
-  cases tl; case _ kl1 kl2 =>
   apply Judgment.allt;
-  apply compile_preserves_kinds kl1 rfl h1 c2 cc;
-  apply @ih1 ★ w2 (.kind w1 :: Γ') .HsType _ _ kl2 c3 _
+  apply compile_preserves_kinds cc h1 c2;
+  apply @ih1 (.kind w1 :: Γ') ★ w2 _ _ _ c3
+  case _ => apply CompileCtx.kind; assumption; assumption; assumption
   case _ => apply HsJudgment.ax; apply HsJudgment.wfkind; assumption; assumption
   case _ => unfold compile_kind; rfl
-  case _ => apply CompileCtx.kind; assumption; assumption
+
 case _ j1 _ j2 ih1 ih2 =>
   rw[Option.bind_eq_some] at c2;
   cases c2; case _ w1 c2 =>
@@ -178,19 +177,21 @@ case _ j1 _ j2 ih1 ih2 =>
   rw[Option.bind_eq_some] at c3;
   cases c3; case _ w2 c3 =>
   cases c3; case _ c3 e =>
-  cases e; cases tl;
-  have lem1 := compile_preserves_kinds kl rfl j1 c1 cc;
+  cases e;
+  have lem1 := compile_preserves_kinds cc j1 c1;
   unfold compile_kind at c1; simp at c1;
   cases j1; simp at c1; cases c1;
-  case _ tl1 tl2 _ =>
   apply Judgment.arrow;
-  apply @ih1 ★ w1 Γ' .HsType _ _ tl1 c2 cc;
+  apply @ih1 Γ' ★ w1 cc _ _;
+  case _ => apply c2;
   case _ => apply HsJudgment.ax; assumption
   case _ => unfold compile_kind; rfl
-  apply @ih2 ★ w2 (.empty::Γ') .HsType _ _ tl2 c3 _
+
+  apply @ih2 (.empty::Γ') ★ w2 _ _ _ c3
+  case _ => apply CompileCtx.empty; assumption; assumption
   case _ => apply HsJudgment.ax; apply HsJudgment.wfempty; assumption
   case _ => unfold compile_kind; rfl
-  case _ => apply CompileCtx.empty; assumption
+
 case _ j1 _ j2 ih1 ih2 =>
   rw[Option.bind_eq_some] at c2;
   cases c2; case _ w1 c2 =>
@@ -198,44 +199,60 @@ case _ j1 _ j2 ih1 ih2 =>
   rw[Option.bind_eq_some] at c3;
   cases c3; case _ w2 c3 =>
   cases c3; case _ c3 e =>
-  cases e; cases tl;
-  have lem1 := compile_preserves_kinds kl rfl j1 c1 cc;
+  cases e;
+  have lem1 := compile_preserves_kinds cc j1 c1;
   unfold compile_kind at c1; simp at c1;
   cases j1; simp at c1; cases c1;
   case _ tl1 tl2 _ =>
   apply Judgment.arrow;
-  apply @ih1 ★ w1 Γ' .HsType _ _ tl1 c2 cc;
+  apply @ih1 Γ' ★ w1 cc _ _ c2;
   case _ => apply HsJudgment.ax; assumption
   case _ => unfold compile_kind; rfl
-  apply @ih2 ★ w2 (.empty::Γ') .HsType _ _ tl2 c3 _
+  apply @ih2 (.empty::Γ') ★ w2 _ _ _ c3
+  case _ => apply CompileCtx.empty; assumption; assumption
   case _ => apply HsJudgment.ax; apply HsJudgment.wfempty; assumption
   case _ => unfold compile_kind; rfl
-  case _ => apply CompileCtx.empty; assumption
-
-inductive HsTermLike : Ctx HsTerm -> HsTerm -> Prop where
-| HsVar : (Γ d@ x).is_ctor || (Γ d@ x).is_type -> HsTermLike Γ `#x
-| HsApp : HsTermLike Γ t1 -> HsTermLike Γ t2 -> HsTermLike Γ (t1 `• t2)
-| HsLam : HsTermLike (.type A :: Γ) t1 -> HsTermLike Γ (`λ{A}t1)
-| HsIte : HsTermLike Γ p -> HsTermLike Γ i -> HsTermLike Γ t -> HsTermLike Γ e -> HsTermLike Γ (.HsIte p i t e)
-| HsLet : HsTypeLike Γ A -> HsTermLike Γ t -> HsTermLike (.term A t :: Γ) t' -> HsTermLike Γ (.HsLet A t t')
-
 
 theorem compile_preserves_typing :
   CompileCtx Γ Γ' ->
-  HsTypeLike Γ τ ->
   (j1 : Γ ⊢τ τ : k) ->
   compile_type Γ τ k j1 = .some τ' ->
-  HsTermLike Γ t ->
   (j2 : Γ ⊢t t : τ) ->
   compile_term Γ t τ j2 = .some t' ->
   Γ' ⊢ t' : τ' := by
-intro cc τl j1 c1 tl j2 c2;
+intro cc j1 c1 j2 c2;
 induction Γ, t, τ, j2 using compile_term.induct generalizing Γ' t' τ' k
-cases tl;
 all_goals (unfold compile_term at c2; simp at c2)
-case _ => cases c2; sorry
-case _ =>
+case _ wf test gt => sorry
+  -- cases c2;
+  -- have lem1 := HsJudgment.var wf test gt
+  -- have lem := compile_preserves_term_indices cc lem1 c1
+  -- apply Judgment.var;
+  -- apply compile_ctx_wf wf cc
+  -- sorry
+case _ j1' j2 j3 ih1 =>
+ rw[Option.bind_eq_some] at c2;
+ cases c2; case _ A' c2 =>
+ cases c2; case _ c2 c3 =>
+ rw[Option.bind_eq_some] at c3;
+ cases c3; case _ t' c3 =>
+ cases c3; case _ c3 e =>
+ cases e;
+ have uniq := typing_uniqueness j1 j3; subst uniq;
+ unfold compile_type at c1; cases j1; simp at c1;
+ rw[Option.bind_eq_some] at c1;
+ cases c1; case _ x1 c1' =>
+ cases c1'; case _ c1' c2' =>
+ rw[Option.bind_eq_some] at c2';
+ cases c2'; case _ B' c2' =>
+ cases c2'; case _ c2' e =>
+ cases e;
+ have e : x1 = A' := by
+   sorry
+ have ih1' := @ih1 (.type A' :: Γ') `★ B' t' sorry sorry sorry c3
+
  sorry
+
 case _ =>
  sorry
 case _ =>
@@ -246,5 +263,22 @@ case _ =>
 -- implicits
 case _ => sorry
 case _ => sorry
+case _ => sorry
+case _ => sorry
+
+
+theorem compile_ctx_wf :
+  CompileCtx Γ Γ' ->
+  ⊢ Γ' := by
+intro h2;
+induction h2;
+case _ => apply Judgment.wfnil
+case _ ih1 =>
+  case _ h1 =>
+  apply Judgment.wfempty; assumption;
+case _ h1 j1 cc ih =>
+ apply Judgment.wfkind;
+ sorry
+ sorry
 case _ => sorry
 case _ => sorry
